Moved lemmas on grows/prefix into trace base

src/core/DY.Core.Trace.Base.fst
@@ -204,6 +204,22 @@ let prefix_grows #label_t tr i =
   reveal_opaque (`%grows) (grows #label_t);
   norm_spec [zeta; delta_only [`%prefix]] (prefix #label_t)
 
+
+/// The relation <$ has Nil as a least element, and
+/// is compatible with growing traces via Snoc
+
+let grows_nil (#label_t:Type) (tr:trace_ label_t)
+  : Lemma (ensures Nil <$ tr)
+    [SMTPat (Nil <$ tr)]
+  = reveal_opaque (`%grows) (grows #label_t)
+
+let grows_snoc (#label_t:Type) (tr:trace_ label_t) (e:trace_entry_ label_t)
+  : Lemma (ensures tr <$ (Snoc tr e))
+    [SMTPat (tr <$ (Snoc tr e))]
+  = reveal_opaque (`%grows) (grows #label_t);
+    norm_spec [zeta; delta_only [`%prefix]] (prefix #label_t)
+
+
 val prefix_prefix_grows:
   #label_t:Type ->
   tr1:trace_ label_t -> tr2:trace_ label_t -> i1:timestamp -> i2:timestamp ->
@@ -253,6 +269,55 @@ let rec prefix_prefix_eq #label_t tr1 tr2 i =
     let Snoc tr2_init _ = tr2 in
     prefix_prefix_eq tr1 tr2_init i
   )
+
+/// Every trace is equal to its full-length prefix
+
+let prefix_full_eq (#label_t:Type) (tr:trace_ label_t)
+  : Lemma (ensures (prefix tr (length tr) == tr))
+    [SMTPat (prefix tr (length tr))]
+  = reveal_opaque (`%prefix) (prefix #label_t);
+    norm_spec [zeta; delta_only [`%prefix]] (prefix #label_t)
+
+/// Two traces with the same length, where one is a prefix of the other, must be the same
+
+let grows_full_eq (#label_t:Type) (tr1 tr2:trace_ label_t)
+  : Lemma
+    (requires tr1 <$ tr2 /\ length tr1 == length tr2)
+    (ensures tr1 == tr2)
+// TODO:
+// It is not clear if this SMTPat is ever practically useful, but it seems like it could be in principle
+    [SMTPat (tr1 == tr2); SMTPat (tr1 <$ tr2)]
+  = prefix_prefix_eq tr1 tr2 (length tr1)
+
+/// The relation <$ is a non-strict partial order, and so if tr1 <$ tr2,
+/// we can split into the case where tr1 and tr2 are equal, and that in which
+/// tr1 is a strict prefix of tr2
+
+let grows_cases (#label_t:Type) (tr1 tr2:trace_ label_t)
+  : Lemma
+    (requires tr1 <$ tr2)
+    (ensures tr1 == tr2 \/ (
+      Snoc? tr2 /\ (
+      let Snoc hd _ = tr2 in
+      tr1 <$ hd
+    )))
+  = if length tr1 = length tr2
+    then grows_full_eq tr1 tr2
+    else begin
+      let open FStar.Calc in
+      let Snoc hd e = tr2 in
+      calc (<$) {
+        tr1;
+        == {}
+        prefix tr1 (length tr1);
+        <$ {}
+        prefix tr2 (length hd);
+        == { assert(hd <$ tr2) } // Triggers prefix_prefix_eq hd tr2 (length hd)
+        prefix hd (length hd);
+        == {}
+        hd;
+      }
+    end
 
 (*** Entries in the trace predicates ***)
 
